refactor examples

examples/load_test.v
@@ -1,23 +1,24 @@
 Require Import isla.base.
 Require Import isla.opsem.
 Require Import isla.automation.
-Require Import isla.instructions.store.
+Require Import isla.instructions.load.
 Require Import isla.examples.sys_regs.
 
 Definition spec `{!islaG Σ} `{!threadG} a : iProp Σ :=
+  ∃ (vold : bv 64),
   "R1" ↦ᵣ Val_Bits [BV{64} 0x0000000000000008] ∗
   [BV{64} 0x0000000000000008] ↦ₘ [BV{64} 0x00000000deadbeef] ∗
-  "R9" ↦ᵣ Val_Bits [BV{64} 0x00000000cafebabe] ∗
+  "R0" ↦ᵣ Val_Bits vold ∗
   reg_col sys_regs ∗
   instr_pre a (
     "R1" ↦ᵣ Val_Bits [BV{64} 0x0000000000000008] ∗
-    [BV{64} 0x0000000000000008] ↦ₘ [BV{64} 0x00000000cafebabe] ∗
-    "R9" ↦ᵣ Val_Bits [BV{64} 0x00000000cafebabe] ∗
+    [BV{64} 0x0000000000000008] ↦ₘ [BV{64} 0x00000000deadbeef] ∗
+    "R0" ↦ᵣ Val_Bits [BV{64} 0x00000000deadbeef] ∗
     reg_col sys_regs ∗
     True).
 
-Lemma store_wp `{!islaG Σ} `{!threadG}:
-  instr 0x0000000010300000 (Some [store_trace]) -∗
+Lemma load_wp `{!islaG Σ} `{!threadG}:
+  instr 0x0000000010300000 (Some [load_trace]) -∗
   instr_body 0x0000000010300000 (spec 0x0000000010300004).
 Proof.
   iStartProof.
