examples/stp_test.v
@@ -2,29 +2,9 @@ Require Import isla.base.
 Require Import isla.opsem.
 Require Import isla.automation.
 Require Import isla.instructions.stp.
+Require Import isla.examples.sys_regs.
 
-Definition start_address := [BV{64} (0x0000000010300000 - 0x4)].
-Definition spec : list seq_label := [ SInstrTrap [BV{64} 0x0000000010300004] ].
-
-Definition sys_regs : list (reg_col_entry * valu) := [
-  (RegColDirect "SCTLR_EL2" , Val_Bits [BV{64} 0x0000000004000002] );
-  (RegColDirect "SCR_EL3" , Val_Bits [BV{32} 0] );
-  (RegColDirect "TCR_EL2" , Val_Bits [BV{64} 0] );
-  (RegColDirect "CFG_ID_AA64PFR0_EL1_EL0" , Val_Bits [BV{4} 1] );
-  (RegColDirect "CFG_ID_AA64PFR0_EL1_EL1" , Val_Bits [BV{4} 1] );
-  (RegColDirect "CFG_ID_AA64PFR0_EL1_EL2" , Val_Bits [BV{4} 1] );
-  (RegColDirect "CFG_ID_AA64PFR0_EL1_EL3" , Val_Bits [BV{4} 1] );
-  (RegColDirect "OSLSR_EL1" , Val_Bits [BV{32} 0] );
-  (RegColDirect "OSDLR_EL1" , Val_Bits [BV{32} 0] );
-  (RegColDirect "EDSCR" , Val_Bits [BV{32} 0] );
-  (RegColDirect "MPIDR_EL1" , Val_Bits [BV{64} 0] );
-  (RegColStruct "PSTATE" "SP" , Val_Bits [BV{1} 1] );
-  (RegColStruct "PSTATE" "EL" , Val_Bits [BV{2} 2] );
-  (RegColStruct "PSTATE" "nRW" , Val_Bits [BV{1} 0] );
-  (RegColStruct "PSTATE" "D" , Val_Bits [BV{1} 1])
-].
-
-Definition cont_spec `{!islaG Σ} `{!threadG} a sp (v1 v2 : bv 64) : iProp Σ :=
+Definition spec `{!islaG Σ} `{!threadG} a sp (v1 v2 : bv 64) : iProp Σ :=
   ∃ (vold1 vold2 : bv 64),
   "R0" ↦ᵣ Val_Bits v1 ∗
   "R1" ↦ᵣ Val_Bits v2 ∗
@@ -44,10 +24,10 @@ Definition cont_spec `{!islaG Σ} `{!threadG} a sp (v1 v2 : bv 64) : iProp Σ :=
 
 Lemma stp_wp `{!islaG Σ} `{!threadG} (sp v1 v2: bv 64):
   instr 0x0000000010300000 (Some [stp_trace]) -∗
-  instr_body 0x0000000010300000 (cont_spec 0x0000000010300004 sp v1 v2).
+  instr_body 0x0000000010300000 (spec 0x0000000010300004 sp v1 v2).
 Proof.
   iStartProof.
-  unfold cont_spec.
+  unfold spec.
   repeat liAStep; liShow.
   Unshelve.
   all: try (repeat f_equal; bv_solve).
